proof/crefine/StateRelation_C.thy
@@ -765,7 +765,7 @@ where
   | SysWait \<Rightarrow> scast Kernel_C.SysWait
   | SysReply \<Rightarrow> scast Kernel_C.SysReply
   | SysReplyWait \<Rightarrow> scast Kernel_C.SysReplyWait
-  | SysPoll \<Rightarrow> scast Kernel_C.SysPoll
+  | SysNBWait \<Rightarrow> scast Kernel_C.SysNBWait
   | SysYield \<Rightarrow> scast Kernel_C.SysYield"
 
 lemma (in kernel) cmap_relation_cs_atD:
