proof/refine/Ipc_R.thy
@@ -3535,13 +3535,22 @@ lemma complete_async_ipc_corres:
   apply (clarsimp simp: projectKOs valid_obj'_def valid_aep'_def obj_at'_def)
   done
 
+
+lemma do_nbwait_failed_transfer_corres:
+  "corres dc (tcb_at thread)
+            (tcb_at' thread)
+            (do_nbwait_failed_transfer thread)
+            (doNBWaitFailedTransfer thread)"
+  unfolding do_nbwait_failed_transfer_def doNBWaitFailedTransfer_def
+  by (simp add: badgeRegister_def badge_register_def, rule user_setreg_corres)
+  
 lemma receive_ipc_corres:
   assumes "is_ep_cap cap" and "cap_relation cap cap'"
   shows "
    corres dc (einvs and valid_sched and tcb_at thread and valid_cap cap and ex_nonz_cap_to thread
               and cte_wp_at (\<lambda>c. c = cap.NullCap) (thread, tcb_cnode_index 3))
              (invs' and tcb_at' thread and valid_cap' cap')
-             (receive_ipc thread cap) (receiveIPC thread cap')"
+             (receive_ipc thread cap isBlocking) (receiveIPC thread cap' isBlocking)"
   apply (insert assms)
   apply (simp add: receive_ipc_def receiveIPC_def
               split del: split_if)
@@ -3570,15 +3579,17 @@ lemma receive_ipc_corres:
                -- "IdleEP"
                apply (simp add: ep_relation_def)
                apply (rule corres_guard_imp)
-                 apply (rule corres_split [OF _ sts_corres])
-                    apply (rule set_ep_corres)
-                    apply (simp add: ep_relation_def)
-            apply simp
-           apply (simp add: valid_pspace_def)
-           apply wp
-         apply (clarsimp simp add: invs_def valid_state_def valid_pspace_def 
-                          valid_tcb_state_def st_tcb_at_tcb_at)
-        apply auto[1]
+                 apply (case_tac isBlocking; simp)
+                  apply (rule corres_split [OF _ sts_corres])
+                     apply (rule set_ep_corres)
+                     apply (simp add: ep_relation_def)
+                    apply simp
+                   apply wp
+                 apply (rule corres_guard_imp, rule do_nbwait_failed_transfer_corres, simp)
+                 apply simp
+                apply (clarsimp simp add: invs_def valid_state_def valid_pspace_def
+               valid_tcb_state_def st_tcb_at_tcb_at)
+               apply auto[1]
        -- "SendEP"
        apply (simp add: ep_relation_def)
        apply (rename_tac list)
@@ -3651,11 +3662,14 @@ lemma receive_ipc_corres:
              -- "RecvEP"
              apply (simp add: ep_relation_def)
              apply (rule_tac corres_guard_imp)
-               apply (rule corres_split [OF _ sts_corres])
-                  apply (rule set_ep_corres)
-                  apply (simp add: ep_relation_def)
-                 apply simp
-                apply wp
+               apply (case_tac isBlocking; simp)
+                apply (rule corres_split [OF _ sts_corres])
+                   apply (rule set_ep_corres)
+                   apply (simp add: ep_relation_def)
+                  apply simp
+                 apply wp
+               apply (rule corres_guard_imp, rule do_nbwait_failed_transfer_corres, simp)
+               apply simp
               apply (clarsimp simp: valid_tcb_state_def)
              apply (clarsimp simp add: valid_tcb_state'_def)
             apply (rule corres_option_split[rotated 2])
@@ -3676,14 +3690,6 @@ lemma receive_ipc_corres:
              dest!: invs_valid_objs' obj_at_valid_objs'
              split: option.splits)
   done
-
-lemma do_poll_failed_transfer_corres:
-  "corres dc (tcb_at thread)
-            (tcb_at' thread)
-            (do_poll_failed_transfer thread)
-            (doPollFailedTransfer thread)"
-  unfolding do_poll_failed_transfer_def doPollFailedTransfer_def
-  by (simp add: badgeRegister_def badge_register_def, rule user_setreg_corres)
 
 lemma receive_async_ipc_corres:
  "\<lbrakk> is_aep_cap cap; cap_relation cap cap' \<rbrakk> \<Longrightarrow>
@@ -3712,7 +3718,7 @@ lemma receive_async_ipc_corres:
               apply (simp add: aep_relation_def)
              apply simp
             apply wp
-          apply (rule corres_guard_imp, rule do_poll_failed_transfer_corres, simp+)
+          apply (rule corres_guard_imp, rule do_nbwait_failed_transfer_corres, simp+)
        -- "WaitingAEP"
        apply (simp add: aep_relation_def)
        apply (rule corres_guard_imp)
@@ -3723,7 +3729,7 @@ lemma receive_async_ipc_corres:
             apply simp
            apply wp
          apply (rule corres_guard_imp)
-           apply (rule do_poll_failed_transfer_corres, simp+)
+           apply (rule do_nbwait_failed_transfer_corres, simp+)
       -- "ActiveAEP"
       apply (simp add: aep_relation_def)
       apply (rule corres_guard_imp)
@@ -4156,7 +4162,7 @@ lemma ri_invs' [wp]:
           and (\<lambda>s. \<forall>p. t \<notin> set (ksReadyQueues s p))
           and ex_nonz_cap_to' t
           and (\<lambda>s. \<forall>r \<in> zobj_refs' cap. ex_nonz_cap_to' r s)\<rbrace>
-  receiveIPC t cap 
+  receiveIPC t cap isBlocking
   \<lbrace>\<lambda>_. invs'\<rbrace>" (is "\<lbrace>?pre\<rbrace> _ \<lbrace>_\<rbrace>")
   apply (clarsimp simp: receiveIPC_def) 
   apply (rule hoare_seq_ext [OF _ get_ep_sp'])
@@ -4168,10 +4174,11 @@ lemma ri_invs' [wp]:
    apply (case_tac ep)
      -- "endpoint = RecvEP"
      apply (simp add: invs'_def valid_state'_def)
-     apply (rule hoare_pre, wp valid_irq_node_lift)
+     apply (rule hoare_pre, wpc, wp valid_irq_node_lift)
       apply (simp add: valid_ep'_def)
       apply (wp sts_sch_act' hoare_vcg_const_Ball_lift valid_irq_node_lift
-                sts_valid_queues setThreadState_ct_not_inQ)
+                sts_valid_queues setThreadState_ct_not_inQ 
+           | simp add: doNBWaitFailedTransfer_def)+
      apply (clarsimp simp: valid_tcb_state'_def pred_tcb_at')
      apply (rule conjI, clarsimp elim!: obj_at'_weakenE)
      apply (frule obj_at_valid_objs')
@@ -4196,10 +4203,11 @@ lemma ri_invs' [wp]:
      apply (fastforce simp: valid_pspace'_def global'_no_ex_cap idle'_not_queued)
    -- "endpoint = IdleEP"
     apply (simp add: invs'_def valid_state'_def)
-    apply (rule hoare_pre, wp valid_irq_node_lift)
+    apply (rule hoare_pre, wpc, wp valid_irq_node_lift)
      apply (simp add: valid_ep'_def)
      apply (wp sts_sch_act' valid_irq_node_lift
-               sts_valid_queues setThreadState_ct_not_inQ)
+               sts_valid_queues setThreadState_ct_not_inQ
+          | simp add: doNBWaitFailedTransfer_def)+
     apply (clarsimp simp: pred_tcb_at' valid_tcb_state'_def)
     apply (rule conjI, clarsimp elim!: obj_at'_weakenE)
     apply (subgoal_tac "t \<noteq> capEPPtr cap")
@@ -4293,7 +4301,7 @@ lemma rai_invs'[wp]:
     apply (rule hoare_pre)
      apply (wp valid_irq_node_lift sts_sch_act' typ_at_lifts
                sts_valid_queues setThreadState_ct_not_inQ
-            | simp add: valid_aep'_def doPollFailedTransfer_def | wpc)+
+            | simp add: valid_aep'_def doNBWaitFailedTransfer_def | wpc)+
     apply (clarsimp simp: pred_tcb_at' valid_tcb_state'_def)
     apply (rule conjI, clarsimp elim!: obj_at'_weakenE)
     apply (subgoal_tac "capAEPPtr cap \<noteq> t")
@@ -4329,7 +4337,7 @@ lemma rai_invs'[wp]:
   apply (rule hoare_pre)
    apply (wp hoare_vcg_const_Ball_lift valid_irq_node_lift sts_sch_act'
              sts_valid_queues setThreadState_ct_not_inQ typ_at_lifts
-        | simp add: valid_aep'_def doPollFailedTransfer_def | wpc)+
+        | simp add: valid_aep'_def doNBWaitFailedTransfer_def | wpc)+
   apply (clarsimp simp: valid_tcb_state'_def)
   apply (frule_tac t=t in not_in_aepQueue)
      apply (simp)
@@ -4778,7 +4786,7 @@ crunch pred_tcb_at'[wp]: switchIfRequiredTo, completeAsyncIPC "pred_tcb_at' proj
 
 lemma ri_makes_runnable_simple':
   "\<lbrace>st_tcb_at' P t' and K (t \<noteq> t') and K (P = runnable' \<or> P = simple')\<rbrace>
-     receiveIPC t epCap
+     receiveIPC t epCap isBlocking
    \<lbrace>\<lambda>rv. st_tcb_at' P t'\<rbrace>"
   apply (rule hoare_gen_asm)+
   apply (simp add: receiveIPC_def)
@@ -4788,7 +4796,7 @@ lemma ri_makes_runnable_simple':
   apply wp
    apply (rename_tac ep q r)
    apply (case_tac ep, simp_all)
-     apply (wp sts_st_tcb_at'_cases)
+     apply (wp sts_st_tcb_at'_cases | wpc | simp add: doNBWaitFailedTransfer_def)+
    apply (rename_tac list)
    apply (case_tac list, simp_all add: case_bool_If case_option_If
                             split del: split_if cong: if_cong)
@@ -4816,7 +4824,7 @@ lemma rai_makes_runnable_simple':
   apply (rule hoare_gen_asm)
   apply (simp add: receiveAsyncIPC_def)
   apply (rule hoare_pre)
-   by (wp sts_st_tcb_at'_cases getAsyncEP_wp | wpc | simp add: doPollFailedTransfer_def)+
+   by (wp sts_st_tcb_at'_cases getAsyncEP_wp | wpc | simp add: doNBWaitFailedTransfer_def)+
 
 lemma sendAsyncIPC_st_tcb'_Running:
   "\<lbrace>st_tcb_at' (\<lambda>st. st = Running \<or> P st) t\<rbrace>
